Adds functional proof for quicksort. (#120)
* Adds functional proof for quicksort.

Proves quicksort_ST and quicksort_fun are equivalent in behavior.

* Make quicksort_ST_list check for empty list.

Then it returns an empty list immediately, as its sorted.

---------

Co-authored-by: ikariniemi <ikariniemi@bloomberg.net>

tests/monadic/stmonad/STMonadExamples.v
@@ -231,11 +231,15 @@ Section NatExampleTrees.
 
     
     Definition quicksort_ST_list (xs : list nat) : itree E0 (list nat) :=
-      let lastIndex := fromNat (length xs - 1) in 
-      arr <- newListArray zero zero lastIndex xs;;
-      quicksort_ST arr zero zero lastIndex;;
-      newXs <- getElems arr;;
-      Ret newXs.
+      match xs with
+      | [] => Ret []
+      | _::_ => 
+        let lastIndex := fromNat (length xs - 1) in 
+        arr <- newListArray zero zero lastIndex xs;;
+        quicksort_ST arr zero zero lastIndex;;
+        newXs <- getElems arr;;
+        Ret newXs
+      end.
   
 
 
@@ -246,21 +250,21 @@ End NatExampleTrees.
 
 
 
-Lemma filter_length {A} (f : A -> bool) (l : list A) :
-  length (List.filter f l) <= length l.
-Proof. induction l; simpl; [lia | destruct (f a); simpl; lia]. Qed.
+  Lemma filter_length {A} (f : A -> bool) (l : list A) :
+    length (List.filter f l) <= length l.
+  Proof. induction l; simpl; [lia | destruct (f a); simpl; lia]. Qed.
 
-Section FunctionalQuicksort.
+  Section FunctionalQuicksort.
 
-  Equations? quicksort_fun (l : list nat) : list nat by wf (length l) lt :=
-    quicksort_fun [] => [];
-    quicksort_fun (p :: xs) =>
-      quicksort_fun (List.filter (fun x => Nat.ltb x p) xs)
-        ++ [p] ++
-      quicksort_fun (List.filter (fun x => Nat.leb p x) xs).
-  - specialize (filter_length (fun x => Nat.ltb x p) xs) as H. lia.   
-  - specialize (filter_length (fun x => Nat.leb p x) xs) as H. lia.   
-  Defined.
+    Equations? quicksort_fun (l : list nat) : list nat by wf (length l) lt :=
+      quicksort_fun [] => [];
+      quicksort_fun (p :: xs) =>
+        quicksort_fun (List.filter (fun x => Nat.ltb x p) xs)
+          ++ [p] ++
+        quicksort_fun (List.filter (fun x => Nat.leb p x) xs).
+    - specialize (filter_length (fun x => Nat.ltb x p) xs) as H. lia.   
+    - specialize (filter_length (fun x => Nat.leb p x) xs) as H. lia.   
+    Defined.
 
 End FunctionalQuicksort.
 
